theories/SetModel/model_interp.v
@@ -3,6 +3,7 @@ From TypedConfluence Require Import core unscoped AST SubstNotations.
 From TypedConfluence Require Import Util BasicAST Contexts Typing. 
 
 Import ListNotations.
+Import CombineNotations.
 
 Require Import library.
 Require Import ZF_axioms ZF_library ZF_nat ZF_acc.
@@ -34,7 +35,7 @@ with nth_proj : forall (Γ : ctx) (l : level) (x : nat), (ZFSet -> ZFSet) -> Pro
              -> nth_proj (Γ ,, (prop , A)) prop 0 (setSndSigma 0 iΓ iA)
 
 | there_irr : forall Γ l A x iΓ iA ix, interp_ctx Γ iΓ -> interp_tm Γ (ty 0) A iA -> nth_proj Γ l x ix
-              -> nth_proj (Γ ,, (prop , A)) l (S x) (fun γa => ix (setFstSigma 0 iΓ iA γa))
+              -> nth_proj (Γ ,, (prop , A)) l (S x) (fun γa => ix (setFstSigma 0 iΓ (fun γ => 𝕌el 0 (boxTy_HO iA γ)) γa))
 
 with interp_tm : forall (Γ : ctx) (l : level) (A : term), (ZFSet -> ZFSet) -> Prop :=
 
@@ -100,10 +101,10 @@ with interp_tm : forall (Γ : ctx) (l : level) (A : term), (ZFSet -> ZFSet) -> P
                   -> interp_tm Γ (ty 0) m im
                   -> interp_tm Γ (ty l) (rec (ty l) P pz ps m) (natrecTm_HO l iP ipz ips im)
 
-| interp_acc : forall Γ i A R a iA iR ia, interp_tm Γ (Ax i) A iA
-               -> interp_tm (Γ ,, (i, A) ,, (i, S ⋅ A)) (Ax prop) R iR
-               -> interp_tm Γ i a ia
-               -> interp_tm Γ (Ax prop) (Core.acc i A R a) (accTy_HO iA iR ia)
+| interp_acc : forall Γ i A R a iA iR ia, interp_tm Γ (Ax (ty i)) A iA
+               -> interp_tm (Γ ,, (ty i, A) ,, (ty i, S ⋅ A)) (Ax prop) R iR
+               -> interp_tm Γ (ty i) a ia
+               -> interp_tm Γ (Ax prop) (Core.acc (ty i) A R a) (accTy_HO iA iR ia)
 
 | interp_accelim : forall Γ i l A R a q P p iA iR ia iP ip, interp_tm Γ (Ax i) A iA
                    -> interp_tm (Γ ,, (i, A) ,, (i, S ⋅ A)) (Ax prop) R iR
@@ -112,12 +113,10 @@ with interp_tm : forall (Γ : ctx) (l : level) (A : term), (ZFSet -> ZFSet) -> P
                    -> interp_tm Γ i a ia
                    -> interp_tm Γ (ty l) (accel i (ty l) A R P p a q) (accelimTm_HO l iA iR iP ip ia)
 
-| interp_obseq_r : forall Γ l A a b iA ia ib, interp_tm Γ (Ax (ty l)) A iA
+| interp_obseq : forall Γ l A a b iA ia ib, interp_tm Γ (Ax (ty l)) A iA
                    -> interp_tm Γ (ty l) a ia
                    -> interp_tm Γ (ty l) b ib
                    -> interp_tm Γ (Ax prop) (obseq (ty l) A a b) (eqTy_HO iA ia ib)
-
-| interp_obseq_i : forall Γ A a b, interp_tm Γ (Ax prop) (obseq prop A a b) (fun _ => ⋆)
 
 | interp_cast : forall Γ l A B e a iA iB ia, interp_tm Γ (Ax (ty l)) A iA
                 -> interp_tm Γ (Ax (ty l)) B iB
@@ -169,7 +168,6 @@ Proof.
   - intros Γ i l A R a q P p iA iR ia iP ip fA IHA fR IHR fP IHP fp IHp fa IHa it ft.
     inversion ft. subst. f_equal ; auto.
   - intros Γ l A a b iA ia ib fA IHA fa IHa fb IHb iP fP. inversion fP. subst. f_equal ; auto.
-  - intros Γ A a b iP fP. now inversion fP. 
   - intros Γ l A B e a iA iB ia fA IHA fB IHB fa IHa it ft.
     inversion ft. subst. f_equal ; auto.
   - intros iΓ fΓ. now inversion fΓ. 
@@ -184,7 +182,7 @@ Proof.
     refine (f_equal3 (fun X Y Z => (fun γa : ZFSet => X (setFstSigma lA Y (fun γ : ZFSet => 𝕌el lA (Z γ)) γa))) _ _ _) ; auto.
   - intros Γ A iΓ iA fΓ IHΓ fA IHA iΔ fΔ. inversion fΔ. subst. f_equal ; auto.
   - intros Γ l A x iΓ iA ix fΓ IHΓ fA IHA fx IHx iy fy. inversion fy. subst.
-    refine (f_equal3 (fun X Y Z => (fun γa : ZFSet => X (setFstSigma 0 Y Z γa))) _ _ _) ; auto.
+    refine (f_equal3 (fun X Y Z => (fun γa : ZFSet => X (setFstSigma 0 Y (fun γ => 𝕌el 0 (boxTy_HO Z γ)) γa))) _ _ _) ; auto.
 Qed.
 
 Lemma functional_tm {Γ l} (t : term) {it it'} : interp_tm Γ l t it -> interp_tm Γ l t it' -> it = it'.
@@ -201,3 +199,227 @@ Lemma functional_nth {Γ l} (x : nat) {ix ix'} : nth_proj Γ l x ix -> nth_proj 
 Proof.
   intros fx fx'. eapply functional_interp. exact fx. exact fx'.
 Qed.
+
+(* The interpretation function only depends on the interpretation of the types in Γ, not really on Γ *)
+(* This could be trivial if we used graphs instead of higher-order functions -- this is the price to
+   pay for a nicer substitution calculus *)
+
+Inductive same_ctx : ctx -> ctx -> Prop :=
+| same_empty : same_ctx ∙ ∙
+
+| same_cons : forall Γ1 Γ2 l A1 A2 iΓ iA1 iA2, same_ctx Γ1 Γ2 
+                  -> interp_ctx Γ1 iΓ -> interp_tm Γ1 (Ax l) A1 iA1 -> interp_tm Γ2 (Ax l) A2 iA2
+                  -> (∀ γ ∈ iΓ, iA1 γ ≡ iA2 γ) -> same_ctx (Γ1 ,, (l , A1)) (Γ2 ,, (l , A2)).
+
+Inductive BoxS (A : SProp) : Prop :=
+| boxS : A -> BoxS A.
+
+Definition is_same_ctx_ctx (Γ : ctx) (iΓ : ZFSet) (fΓ : interp_ctx Γ iΓ) : Prop :=
+  BoxS (forall Γ' iΓ', same_ctx Γ Γ' -> interp_ctx Γ' iΓ' -> iΓ ≡ iΓ').
+
+Definition is_same_ctx_tm (Γ : ctx) (l : level) (t : term) (it : ZFSet -> ZFSet) (ft : interp_tm Γ l t it) : Prop :=
+  BoxS (forall Γ' iΓ it', same_ctx Γ Γ' -> interp_ctx Γ iΓ -> interp_tm Γ' l t it' -> forall γ, γ ∈ iΓ -> it γ ≡ it' γ).
+
+Definition is_same_ctx_proj (Γ : ctx) (l : level) (x : nat) (ix : ZFSet -> ZFSet) (fx : nth_proj Γ l x ix) : Prop :=
+  BoxS (forall Γ' iΓ ix', same_ctx Γ Γ' -> interp_ctx Γ iΓ -> nth_proj Γ' l x ix' -> forall γ, γ ∈ iΓ -> ix γ ≡ ix' γ).
+
+Lemma is_same_ctx : (forall Γ l t it ft, is_same_ctx_tm Γ l t it ft)
+                    /\ (forall Γ iΓ fΓ, is_same_ctx_ctx Γ iΓ fΓ)
+                    /\ (forall Γ l x ix fx, is_same_ctx_proj Γ l x ix fx).
+Proof.
+  apply interp_mutind.
+  - intros Γ l x ix fx IHx. apply boxS. intros Γ' iΓ it' HΓΓ' fΓ ft'. inversion ft' ; subst ; clear ft'.
+    destruct IHx as [ IHx ]. apply (IHx Γ' iΓ it' HΓΓ' fΓ H2).
+  - intros Γ l. apply boxS. intros Γ' iΓ it' HΓΓ' fΓ ft'. inversion ft' ; subst ; clear ft'. easy.
+  - intros Γ. apply boxS. intros Γ' iΓ it' HΓΓ' fΓ ft'. inversion ft' ; subst ; clear ft'. easy.
+  - intros Γ lA lB A B iA iB fA IHA fB IHB. apply boxS. intros Γ' iΓ it' HΓΓ' fΓ ft'.
+    destruct IHA as [ IHA ]. destruct IHB as [ IHB ]. inversion ft' ; subst ; clear ft'. 
+    assert (∀ γ ∈ iΓ, iA γ ≡ iA0 γ) as HAA0. now apply (IHA Γ').
+    assert (∀ γa ∈ ctxExt lA iΓ iA, iB γa ≡ iB0 γa) as HBB0.
+    { refine (IHB (Γ',, (ty lA, A)) (ctxExt lA iΓ iA) iB0 _ _ _).
+      - apply (same_cons Γ Γ' (ty lA) A A iΓ iA iA0 HΓΓ' fΓ fA H6 HAA0).
+      - now eapply interp_cons_rel.
+      - exact H7. }
+    now apply piTy_HO_cong.
+  - intros Γ lB A B iA iB fA IHA fB IHB. apply boxS. intros Γ' iΓ it' HΓΓ' fΓ ft'.
+    destruct IHA as [ IHA ]. destruct IHB as [ IHB ]. inversion ft' ; subst ; clear ft'. 
+    assert (∀ γ ∈ iΓ, iA γ ≡ iA0 γ) as HAA0. now apply (IHA Γ').
+    assert (∀ γa ∈ ctxExt 0 iΓ (boxTy_HO iA), iB γa ≡ iB0 γa) as HBB0.
+    { refine (IHB (Γ',, (prop, A)) (ctxExt 0 iΓ (boxTy_HO iA)) iB0 _ _ _).
+      - refine (same_cons Γ Γ' prop A A iΓ iA iA0 HΓΓ' fΓ fA H3 HAA0).
+      - now eapply interp_cons_irr.
+      - exact H5. }
+    apply piTy_HO_cong. unfold boxTy_HO. intros γ Hγ. destruct (HAA0 γ Hγ). reflexivity. exact HBB0.
+  - intros Γ lA A B iA iB fA IHA fB IHB. apply boxS. intros Γ' iΓ it' HΓΓ' fΓ ft'.
+    destruct IHA as [ IHA ]. destruct IHB as [ IHB ]. inversion ft' ; subst ; clear ft'. 
+    assert (∀ γ ∈ iΓ, iA γ ≡ iA0 γ) as HAA0. now apply (IHA Γ').
+    assert (∀ γa ∈ ctxExt lA iΓ iA, iB γa ≡ iB0 γa) as HBB0.
+    { refine (IHB (Γ',, (ty lA, A)) (ctxExt lA iΓ iA) iB0 _ _ _).
+      - apply (same_cons Γ Γ' (ty lA) A A iΓ iA iA0 HΓΓ' fΓ fA H3 HAA0).
+      - now eapply interp_cons_rel.
+      - exact H5. }
+    now apply forallTy_HO_cong. 
+  - intros Γ A B iA iB fA IHA fB IHB. apply boxS. intros Γ' iΓ it' HΓΓ' fΓ ft'.
+    destruct IHA as [ IHA ]. destruct IHB as [ IHB ]. inversion ft' ; subst ; clear ft'. 
+    assert (∀ γ ∈ iΓ, iA γ ≡ iA0 γ) as HAA0. now apply (IHA Γ').
+    assert (∀ γa ∈ ctxExt 0 iΓ (boxTy_HO iA), iB γa ≡ iB0 γa) as HBB0.
+    { refine (IHB (Γ',, (prop, A)) (ctxExt 0 iΓ (boxTy_HO iA)) iB0 _ _ _).
+      - refine (same_cons Γ Γ' prop A A iΓ iA iA0 HΓΓ' fΓ fA H2 HAA0).
+      - now eapply interp_cons_irr.
+      - exact H3. }
+    apply forallTy_HO_cong. unfold boxTy_HO. intros γ Hγ. destruct (HAA0 γ Hγ). reflexivity. exact HBB0.
+  - intros Γ lA lB A B t iA it fA IHA ft IHt. apply boxS. intros Γ' iΓ it' HΓΓ' fΓ ft'.
+    destruct IHA as [ IHA ]. destruct IHt as [ IHt ]. inversion ft' ; subst ; clear ft'. 
+    assert (∀ γ ∈ iΓ, iA γ ≡ iA0 γ) as HAA0. now apply (IHA Γ').
+    assert (∀ γa ∈ ctxExt lA iΓ iA, it γa ≡ it0 γa) as Htt0.
+    { refine (IHt (Γ',, (ty lA, A)) (ctxExt lA iΓ iA) it0 _ _ _).
+      - refine (same_cons Γ Γ' (ty lA) A A iΓ iA iA0 HΓΓ' fΓ fA H7 HAA0).
+      - now eapply interp_cons_rel.
+      - exact H8. }
+    now apply lamTm_HO_cong.
+  - intros Γ lB A B t iA it fA IHA ft IHt. apply boxS. intros Γ' iΓ it' HΓΓ' fΓ ft'.
+    destruct IHA as [ IHA ]. destruct IHt as [ IHt ]. inversion ft' ; subst ; clear ft'. 
+    assert (∀ γ ∈ iΓ, iA γ ≡ iA0 γ) as HAA0. now apply (IHA Γ').
+    assert (∀ γa ∈ ctxExt 0 iΓ (boxTy_HO iA), it γa ≡ it0 γa) as Htt0.
+    { refine (IHt (Γ',, (prop, A)) (ctxExt 0 iΓ (boxTy_HO iA)) it0 _ _ _).
+      - refine (same_cons Γ Γ' prop A A iΓ iA iA0 HΓΓ' fΓ fA H5 HAA0).
+      - now eapply interp_cons_irr.
+      - exact H6. }
+    apply lamTm_HO_cong. unfold boxTy_HO. intros γ Hγ. destruct (HAA0 γ Hγ). reflexivity. exact Htt0.
+  - intros Γ lA lB A B t u iA it iu fA IHA ft IHt fu IHu. apply boxS. intros Γ' iΓ it' HΓΓ' fΓ ft'.
+    destruct IHA as [ IHA ]. destruct IHt as [ IHt ]. destruct IHu as [ IHu ]. inversion ft' ; subst ; clear ft'. 
+    assert (∀ γ ∈ iΓ, iA γ ≡ iA0 γ) as HAA0. now apply (IHA Γ').
+    assert (∀ γ ∈ iΓ, it γ ≡ it0 γ) as Htt0. now apply (IHt Γ').
+    assert (∀ γ ∈ iΓ, iu γ ≡ iu0 γ) as Huu0. now apply (IHu Γ').
+    now apply appTm_HO_cong.
+  - intros Γ lB A B t u iA it iu fA IHA ft IHt fu IHu. apply boxS. intros Γ' iΓ it' HΓΓ' fΓ ft'.
+    destruct IHA as [ IHA ]. destruct IHt as [ IHt ]. destruct IHu as [ IHu ]. inversion ft' ; subst ; clear ft'. 
+    assert (∀ γ ∈ iΓ, iA γ ≡ iA0 γ) as HAA0. now apply (IHA Γ').
+    assert (∀ γ ∈ iΓ, it γ ≡ it0 γ) as Htt0. now apply (IHt Γ').
+    assert (∀ γ ∈ iΓ, iu γ ≡ iu0 γ) as Huu0. now apply (IHu Γ').
+    apply appTm_HO_cong. unfold boxTy_HO. intros γ Hγ. destruct (HAA0 γ Hγ). reflexivity. exact Htt0. exact Huu0.
+  - intros Γ. apply boxS. intros Γ' iΓ it' HΓΓ' fΓ ft'. inversion ft' ; subst ; clear ft'. easy.
+  - intros Γ. apply boxS. intros Γ' iΓ it' HΓΓ' fΓ ft'. inversion ft' ; subst ; clear ft'. easy.
+  - intros Γ t it ft IHt. apply boxS. intros Γ' iΓ it' HΓΓ' fΓ ft'. inversion ft' ; subst ; clear ft'.
+    destruct IHt as [ IHt ]. assert (∀ γ ∈ iΓ, it γ ≡ it0 γ) as Htt0. now apply (IHt Γ').
+    unfold sucTm_HO. intros γ Hγ. destruct (Htt0 γ Hγ). reflexivity.
+  - intros Γ l P pz ps m iP ipz ips im fP IHP fpz IHpz fps IHps fm IHm. apply boxS. intros Γ' iΓ it' HΓΓ' fΓ ft'.
+    destruct IHP as [ IHP ]. destruct IHpz as [ IHpz ]. destruct IHps as [ IHps ]. destruct IHm as [ IHm ].
+    inversion ft' ; subst ; clear ft'.
+    assert (∀ γa ∈ ctxExt 0 iΓ natTy_HO, iP γa ≡ iP0 γa) as HPP0.
+    { refine (IHP (Γ',, (ty 0, Nat)) (ctxExt 0 iΓ natTy_HO) iP0 _ _ _).
+      - refine (same_cons Γ Γ' (ty 0) Nat Nat iΓ natTy_HO natTy_HO HΓΓ' fΓ _ _ _).
+        + now apply interp_nat.
+        + now apply interp_nat.
+        + intros ; reflexivity.
+      - apply interp_cons_rel. exact fΓ. now apply interp_nat.
+      - exact H5. }
+    assert (∀ γ ∈ iΓ, ipz γ ≡ ipz0 γ) as Hpzpz0. now apply (IHpz Γ').
+    assert (∀ γ ∈ iΓ, im γ ≡ im0 γ) as Hmm0. now apply (IHm Γ').
+    assert (∀ γaa ∈ ctxExt l (ctxExt 0 iΓ natTy_HO) iP, ips γaa ≡ ips0 γaa) as Hpsps0.
+    { refine (IHps (Γ',, (ty 0, Nat),, (ty l, P)) (ctxExt l (ctxExt 0 iΓ natTy_HO) iP) ips0 _ _ _).
+      - refine (same_cons (Γ,, (ty 0, Nat)) (Γ',, (ty 0, Nat)) (ty l) P P _ iP iP0 _ _ _ _ _).
+        + refine (same_cons Γ Γ' (ty 0) Nat Nat iΓ natTy_HO natTy_HO HΓΓ' fΓ _ _ _).
+          * now apply interp_nat.
+          * now apply interp_nat.
+          * intros ; reflexivity.
+        + apply interp_cons_rel. exact fΓ. now apply interp_nat.
+        + exact fP.
+        + exact H5.
+        + apply HPP0.
+      - apply interp_cons_rel.
+        + apply interp_cons_rel. exact fΓ. now apply interp_nat.
+        + exact fP.
+      - exact H8. }
+    now apply natrecTm_HO_cong.
+  - intros Γ i A R a iA iR ia fA IHA fR IHR fa IHa. apply boxS. intros Γ' iΓ it' HΓΓ' fΓ ft'.
+    destruct IHA as [ IHA ]. destruct IHR as [ IHR ]. destruct IHa as [ IHa ]. 
+    inversion ft' ; subst ; clear ft'.
+    assert (∀ γ ∈ iΓ, iA γ ≡ iA0 γ) as HAA0. now apply (IHA Γ').
+    assert (∀ γ ∈ iΓ, ia γ ≡ ia0 γ) as Haa0. now apply (IHa Γ').
+    assert (∀ γaa ∈ ctxExt2 i iΓ iA, iR γaa ≡ iR0 γaa) as HRR0.
+    { refine (IHR (Γ',, (ty i, A),, (ty i, S ⋅ A)) (ctxExt2 i iΓ iA) iR0 _ _ _).
+      - refine (same_cons (Γ,, (ty i, A)) (Γ',, (ty i, A)) (ty i) (S ⋅ A) (S ⋅ A) _ (fun γa => iA (ctx_wk i iΓ iA γa)) (fun γa => iA0 (ctx_wk i iΓ iA0 γa)) _ _ _ _ _).
+        + refine (same_cons Γ Γ' (ty i) A A iΓ iA iA0 HΓΓ' fΓ fA H4 HAA0).
+        + apply interp_cons_rel. exact fΓ. exact fA.
+        + admit.
+        + admit.
+        + intros γa Hγa. apply HAA0. unfold ctx_wk. apply setFstSigma_typing.
+          * intros ; now apply 𝕌el_typing'.
+          * refine (transpS (fun X => γa ∈ X) _ Hγa). apply setSigma_cong.
+            intros γ Hγ. refine (fequal (𝕌el i) _). now apply HAA0.
+      - apply interp_cons_rel.
+        + now apply interp_cons_rel. 
+        + admit.
+      - exact H6. }
+    eapply accTy_HO_cong. exact HAA0. exact HRR0. exact Haa0.
+  - admit.
+  - intros Γ l A a b iA ia ib fA IHA fa IHa fb IHb. apply boxS. intros Γ' iΓ it' HΓΓ' fΓ ft'.
+    destruct IHA as [ IHA ]. destruct IHa as [ IHa ]. destruct IHb as [ IHb ]. inversion ft' ; subst ; clear ft'. 
+    assert (∀ γ ∈ iΓ, ia γ ≡ ia0 γ) as Haa0. now apply (IHa Γ').
+    assert (∀ γ ∈ iΓ, ib γ ≡ ib0 γ) as Hbb0. now apply (IHb Γ').
+    now apply eqTy_HO_cong.
+  - intros Γ l A B e a iA iB ia fA IHA fB IHB fa IHa. apply boxS. intros Γ' iΓ it' HΓΓ' fΓ ft'.
+    destruct IHa as [ IHa ]. inversion ft' ; subst ; clear ft'. 
+    assert (∀ γ ∈ iΓ, ia γ ≡ ia0 γ) as Haa0. now apply (IHa Γ').
+    exact Haa0.
+  - apply boxS. intros Γ' iΓ' HΓΓ' fΓ'. inversion HΓΓ' ; subst ; clear HΓΓ'.
+    inversion fΓ' ; subst ; clear fΓ'. reflexivity.
+  - intros Γ l A iΓ iA fΓ IHΓ fA IHA. apply boxS. intros Γ' iΓ' HΓΓ' fΓ'.
+    destruct IHΓ as [ IHΓ ]. destruct IHA as [ IHA ].
+    inversion HΓΓ' ; subst ; clear HΓΓ'. destruct (functional_ctx Γ fΓ H3) ; clear H3.
+    destruct (functional_tm A fA H4) ; clear H4. inversion fΓ' ; subst ; clear fΓ'.
+    destruct (functional_tm A2 H6 H5) ; clear H5.    
+    assert (iΓ ≡ iΓ0) as HΓΓ0. now apply (IHΓ Γ2). destruct HΓΓ0.
+    unfold ctxExt. apply setSigma_cong. intros γ Hγ. refine (fequal (𝕌el l) _). now apply H7.
+  - intros Γ A iΓ iA fΓ IHΓ fA IHA. apply boxS. intros Γ' iΓ' HΓΓ' fΓ'.
+    destruct IHΓ as [ IHΓ ]. destruct IHA as [ IHA ].
+    inversion HΓΓ' ; subst ; clear HΓΓ'. destruct (functional_ctx Γ fΓ H3) ; clear H3.
+    destruct (functional_tm A fA H4) ; clear H4. inversion fΓ' ; subst ; clear fΓ'.
+    destruct (functional_tm A2 H6 H4) ; clear H4.
+    assert (iΓ ≡ iΓ0) as HΓΓ0. now apply (IHΓ Γ2). destruct HΓΓ0.
+    unfold ctxExt. apply setSigma_cong. intros γ Hγ. unfold boxTy_HO.
+    refine (fequal (fun X => 𝕌el 0 ⟨ X ; _ ⟩) _). now apply H7.
+  - intros Γ l A iΓ iA fΓ IHΓ fA IHA. apply boxS. intros Γ' iΓ' ix HΓΓ' fΓ' fx.
+    destruct IHΓ as [ IHΓ ]. destruct IHA as [ IHA ].
+    inversion fx ; subst ; clear fx. inversion HΓΓ' ; subst ; clear HΓΓ'.
+    destruct (functional_ctx Γ fΓ H7) ; clear H7. destruct (functional_tm A0 H2 H9) ; clear H9.
+    destruct (functional_tm A fA H8) ; clear H8. inversion fΓ' ; subst ; clear fΓ'.
+    destruct (functional_ctx Γ fΓ H5) ; clear H5. destruct (functional_tm A fA H7) ; clear H7.
+    assert (iΓ ≡ iΓ0) as HΓΓ0. now apply (IHΓ Γ0). destruct HΓΓ0. intros γ Hγ.
+    unfold setSndSigma. refine (fequal (fun X => setSndPair iΓ X γ) _). apply setFamUnion_cong.
+    clear γ Hγ. intros γ Hγ. refine (fequal (𝕌el l) _). now apply H10.
+  - intros Γ l lA A x iΓ iA ix fΓ IHΓ fA IHA fx IHx. apply boxS. intros Γ' iΓ' ix' HΓΓ' fΓ' fx'.
+    destruct IHΓ as [ IHΓ ]. destruct IHA as [ IHA ]. destruct IHx as [ IHx ].
+    inversion HΓΓ' ; subst ; clear HΓΓ'. inversion fx' ; subst ; clear fx'. 
+    destruct (functional_ctx Γ fΓ H3) ; clear H3. destruct (functional_tm A2 H6 H11) ; clear H11.
+    destruct (functional_tm A fA H4) ; clear H4. inversion fΓ' ; subst ; clear fΓ'.
+    destruct (functional_ctx Γ fΓ H4) ; clear H4. destruct (functional_tm A fA H5) ; clear H5.
+    assert (iΓ ≡ iΓ1) as HΓΓ0. now apply (IHΓ Γ2). destruct HΓΓ0.
+    assert (∀ γ ∈ iΓ, ix γ ≡ ix0 γ) as Hxx0. now apply (IHx Γ2). intros γ Hγ.
+    assert ((setFstSigma lA iΓ (fun γ0 : ZFSet => 𝕌el lA (iA γ0)) γ) ≡ (setFstSigma lA iΓ (fun γ0 : ZFSet => 𝕌el lA (iA2 γ0)) γ)).
+    { unfold setFstSigma. refine (fequal (fun X => setFstPair iΓ X γ) _). apply setFamUnion_cong.
+      clear γ Hγ. intros γ Hγ. refine (fequal (𝕌el lA) _). now apply H7. } destruct H. apply Hxx0.
+    unfold setFstSigma. apply setFstPair_typing. apply ZFincomp in Hγ. now destruct Hγ.
+  - intros Γ A iΓ iA fΓ IHΓ fA IHA. apply boxS. intros Γ' iΓ' ix HΓΓ' fΓ' fx.
+    destruct IHΓ as [ IHΓ ]. destruct IHA as [ IHA ].
+    inversion fx ; subst ; clear fx. inversion HΓΓ' ; subst ; clear HΓΓ'.
+    destruct (functional_ctx Γ fΓ H7) ; clear H7. destruct (functional_tm A0 H0 H9) ; clear H9.
+    destruct (functional_tm A fA H8) ; clear H8. inversion fΓ' ; subst ; clear fΓ'.
+    destruct (functional_ctx Γ fΓ H3) ; clear H3. destruct (functional_tm A fA H5) ; clear H5.
+    assert (iΓ ≡ iΓ0) as HΓΓ0. now apply (IHΓ Γ0). destruct HΓΓ0. intros γ Hγ.
+    unfold setSndSigma. refine (fequal (fun X => setSndPair iΓ X γ) _). now apply setFamUnion_cong.
+  - intros Γ l A x iΓ iA ix fΓ IHΓ fA IHA fx IHx. apply boxS. intros Γ' iΓ' ix' HΓΓ' fΓ' fx'.
+    destruct IHΓ as [ IHΓ ]. destruct IHA as [ IHA ]. destruct IHx as [ IHx ].
+    inversion HΓΓ' ; subst ; clear HΓΓ'. inversion fx' ; subst ; clear fx'. 
+    destruct (functional_ctx Γ fΓ H3) ; clear H3. destruct (functional_tm A2 H6 H9) ; clear H9.
+    destruct (functional_tm A fA H4) ; clear H4. inversion fΓ' ; subst ; clear fΓ'.
+    destruct (functional_ctx Γ fΓ H1) ; clear H1. destruct (functional_tm A fA H4) ; clear H4.
+    assert (iΓ ≡ iΓ1) as HΓΓ0. now apply (IHΓ Γ2). destruct HΓΓ0.
+    assert (∀ γ ∈ iΓ, ix γ ≡ ix0 γ) as Hxx0. now apply (IHx Γ2). intros γ Hγ.
+    assert ((setFstSigma 0 iΓ iA γ) ≡ (setFstSigma 0 iΓ iA2 γ)).
+    { unfold setFstSigma. refine (fequal (fun X => setFstPair iΓ X γ) _). now apply setFamUnion_cong. }
+    destruct H. apply Hxx0. unfold setFstSigma. apply setFstPair_typing. apply ZFincomp in Hγ. 
+    destruct Hγ as [ Hγ _ ]. refine (transpS (fun X => γ ∈ iΓ × X) _ Hγ). apply setFamUnion_cong.
+    clear γ Hγ. intros γ Hγ. unfold 𝕌el. unfold boxTy_HO. now destruct (H7 γ Hγ).
+Admitted.    
