theories/SetModel/HO_acc.v
@@ -10,6 +10,12 @@ Definition ctxExt2 (n : nat) (Γ : ZFSet) (A : ZFSet -> ZFSet) : ZFSet :=
 Definition accTy_HO (A R a : ZFSet -> ZFSet) : ZFSet -> ZFSet :=
   fun γ => subsingl (acc (A γ) (fun x y => ∅ ∈ R ⟨ ⟨ γ ; y ⟩ ; x ⟩) (a γ)).
 
+Lemma accTy_HO_cong {n : nat} {Γ : ZFSet} {A1 A2 R1 R2 a1 a2 : ZFSet -> ZFSet}
+  (HAe : ∀ γ ∈ Γ, A1 γ ≡ A2 γ) (HRe : ∀ γaa ∈ ctxExt2 n Γ A1, R1 γaa ≡ R2 γaa) (Hae : ∀ γ ∈ Γ, a1 γ ≡ a2 γ) :
+  ∀ γ ∈ Γ, accTy_HO A1 R1 a1 γ ≡ accTy_HO A2 R2 a2 γ.
+Proof.
+Admitted.
+
 Lemma accTy_HO_typing {n : nat} {Γ : ZFSet} {A R a : ZFSet -> ZFSet}
   (HA : ∀ γ ∈ Γ, A γ ∈ 𝕌 n) (HR : ∀ γaa ∈ ctxExt2 n Γ A, R γaa ∈ Ω)
   (Ha : ∀ γ ∈ Γ, a γ ∈ 𝕌el n (A γ)) :
