theories/SetModel/HO_obseq.v
@@ -8,6 +8,13 @@ Require Import HO HO_prop HO_univ HO_forall HO_nat HO_pi HO_box.
 Definition eqTy_HO (A t u : ZFSet -> ZFSet) : ZFSet -> ZFSet :=
   fun γ => subsingl (t γ ≡ u γ).
 
+Lemma eqTy_HO_cong {Γ : ZFSet} {A1 A2 a1 a2 b1 b2 : ZFSet -> ZFSet} 
+  (Hae : ∀ γ ∈ Γ, a1 γ ≡ a2 γ) (Hbe : ∀ γ ∈ Γ, b1 γ ≡ b2 γ) :
+  ∀ γ ∈ Γ, eqTy_HO A1 a1 b1 γ ≡ eqTy_HO A2 a2 b2 γ.
+Proof.
+  intros γ Hγ. unfold eqTy_HO. destruct (Hae γ Hγ). destruct (Hbe γ Hγ). reflexivity.
+Qed.
+
 Lemma eqTy_HO_typing {n : nat} {Γ : ZFSet} {A t u : ZFSet -> ZFSet}
   (HA : ∀ γ ∈ Γ, A γ ∈ 𝕌 n) (Ht : ∀ γ ∈ Γ, t γ ∈ 𝕌el n (A γ)) (Hu : ∀ γ ∈ Γ, u γ ∈ 𝕌el n (A γ)) :
   ∀ γ ∈ Γ, eqTy_HO A t u γ ∈ Ω.
